add for_1_1

VST-introduction/pointer_comparison.c
@@ -40,6 +40,27 @@ int while_1_1(int n) {
     return s;
 }
 
+int for_1_1(int n) {
+    int s;
+    for (s = 0; s <= n; s++) {
+        // No body needed, since the increment happens in the for loop
+    }
+    return s;
+}
+
+// working in progress
+
+
+//
+
+int while_1_2(int n) {
+    int s = 0;
+    while (s + PGSIZE <= n) { // plus
+        s = s + PGSIZE;
+    }
+    return s;
+}
+
 // wokring in progress
 
 
